finished ContainerAxioms proofs

examples/containers/theories/MapProofs.v
@@ -5418,6 +5418,8 @@ Qed.
 
 (** ** Verification of [partition] *)
 
+Set Bullet Behavior "Strict Subproofs".
+
 Lemma partitionWithKey_Bounded:
   forall p map lb ub,
   Bounded map lb ub ->
@@ -5444,17 +5446,23 @@ Proof.
         -- applyDesc link_Desc.
 Qed.
 
+Lemma equal_f : forall {A B : Type} {f g : A -> B},
+  f = g -> forall x, f x = g x.
+Proof.
+  intros. rewrite H. reflexivity.
+Qed.
+
 Lemma partitionWithKey_spec:
   forall (p : e -> a -> bool) map lb ub,
   Bounded map lb ub ->
   Proper ((fun i j : e => i == j = true) ==> eq) p ->
   forall (P : (Map e a * Map e a) -> Prop),
   (forall m1 m2,
-    Desc' m1 lb ub (fun i => match sem m1 i with
+    Desc' m1 lb ub (fun i => match sem map i with
                              | Some y => if p i y then Some y else None
                              | None => None
                               end)  /\
-    Desc' m2 lb ub (fun i => match sem m2 i with
+    Desc' m2 lb ub (fun i => match sem map i with
                              | Some y => if p i y then None else Some y
                              | None => None
                              end) ->
@@ -5474,51 +5482,20 @@ Proof.
     destruct (p x) eqn:?.
     - intros X HX; apply HX; clear X HX; split.
       + destruct_ptrEq.
-        -- solve_Desc. f_solver.
-            **  destruct (sem sl1 i). destruct (p i a1) eqn : ?. inversion Hsem; subst. rewrite Heqb1 in Heqb0.
-                discriminate Heqb0. discriminate Hsem. discriminate Hsem.
-            **  assert (p i v = true). { erewrite HProper. apply Heqb. apply Heqb0. } rewrite H1 in Heqb1.
-                discriminate Heqb1.
-            **  destruct (sem sr1 i). destruct (p i a1) eqn : ?. inversion Hsem1; subst. rewrite Heqb2 in Heqb1.
-                discriminate Heqb1. discriminate Hsem1. discriminate Hsem1.
-        -- applyDesc link_Desc.
-           solve_Desc. f_solver. 
-            ** destruct (sem sl1 i). destruct (p i a1) eqn : ?. inversion Hsem; subst. rewrite Heqb1 in Heqb0.
-               discriminate Heqb0. discriminate Hsem. discriminate Hsem.
-            ** assert (p i a0 = true). { erewrite HProper. apply Heqb. apply Heqb1. } rewrite H1 in Heqb0.
-               discriminate Heqb0.
-            ** destruct (sem sr1 i). destruct (p i a1) eqn : ?; rewrite Hsem3 in Hsem1. inversion Hsem1; subst.
-               rewrite Heqb0 in Heqb2. discriminate Heqb2. discriminate Hsem1. rewrite Hsem3 in Hsem1. 
-              discriminate Hsem1.
-      + applyDesc link2_Desc.
-        solve_Desc. f_solver.
-        -- destruct (sem sl2 i). destruct ( p i a1) eqn : ?. discriminate Hsem0. inversion Hsem0; subst.
-          rewrite Heqb0 in Heqb1. discriminate Heqb1. discriminate Hsem0.
-        -- rewrite Hsem3 in Hsem2. destruct (sem sr2 i). destruct (p i a1) eqn : ?; inversion Hsem2; subst.
-           rewrite Heqb0 in Heqb1. discriminate Heqb1. discriminate Hsem2.
+        -- solve_Desc. f_solver. assert (p i v = p x v). apply equal_f. apply HProper. assumption.
+            rewrite Heqb in H1. rewrite Heqb1 in H1. inversion H1.
+        -- applyDesc link_Desc. solve_Desc. f_solver. assert (p i a0 = p x a0). apply equal_f.
+           apply HProper. assumption. rewrite Heqb1 in H1. rewrite Heqb in H1. inversion H1.
+      + applyDesc link2_Desc. solve_Desc. f_solver. assert (p i v = p x v). apply equal_f.
+        apply HProper. assumption. rewrite Heqb in H3. rewrite Heqb1 in H3. inversion H3.
     - intros X HX; apply HX; clear X HX; split.
-      + applyDesc link2_Desc.
-        solve_Desc. f_solver.
-        -- destruct (sem sl1 i). destruct (p i a1) eqn : ?. inversion Hsem; subst. rewrite Heqb0 in Heqb1.
-          discriminate Heqb1. discriminate Hsem. discriminate Hsem.
-        -- rewrite Hsem3 in Hsem1. destruct (sem sr1 i). destruct (p i a1) eqn : ?; inversion Hsem1; subst.
-            rewrite Heqb0 in Heqb1. discriminate Heqb1. inversion Hsem1.
+      + applyDesc link2_Desc. solve_Desc. f_solver. assert (p i v = p x v). apply equal_f.
+        apply HProper. assumption. rewrite Heqb in H3. rewrite Heqb1 in H3. inversion H3.
       + destruct_ptrEq.
-        -- solve_Desc. f_solver.
-           ** destruct (sem sl2 i). destruct (p i a1) eqn : ?; inversion Hsem0; subst. rewrite Heqb0 in Heqb1.
-              inversion Heqb1. inversion Hsem0.
-           ** assert (p x v = true). { erewrite HProper. apply Heqb1. apply Eq_Symmetric. apply Heqb0. }
-              rewrite Heqb in H1. inversion H1.
-           ** destruct (sem sr2 i). destruct (p i a1) eqn : ?; inversion Hsem2; subst. rewrite Heqb1 in Heqb2.
-              inversion Heqb2. inversion Hsem2.
-        -- applyDesc link_Desc.
-           solve_Desc. f_solver.
-          ** destruct (sem sl2 i). destruct (p i a1) eqn : ?; inversion Hsem0; subst. rewrite Heqb0 in Heqb1.
-            inversion Heqb1. inversion Hsem0.
-          ** assert (p x a0 = true). { erewrite HProper. apply Heqb0. apply Eq_Symmetric.
-             apply Heqb1. } rewrite H1 in Heqb. inversion Heqb.
-          ** rewrite Hsem3 in Hsem2. destruct (sem sr2 i). destruct (p i a1) eqn : ?; inversion Hsem2; subst.
-             rewrite Heqb0 in Heqb2. inversion Heqb2. inversion Hsem2. 
+        -- solve_Desc. f_solver. assert (p x v = p i v). apply equal_f. apply HProper. order e.
+           rewrite Heqb in H1. rewrite Heqb1 in H1. inversion H1.
+        -- applyDesc link_Desc. solve_Desc. f_solver. assert (p x a0 = p i a0). apply equal_f.
+           apply HProper. order e. rewrite Heqb in H1. rewrite Heqb1 in H1. inversion H1.
 Qed.
 
 Lemma partition_spec:
@@ -5526,11 +5503,11 @@ Lemma partition_spec:
   Bounded map lb ub ->
   forall (P : (Map e a * Map e a) -> Prop),
   (forall m1 m2,
-    Desc' m1 lb ub (fun i => match sem m1 i with
+    Desc' m1 lb ub (fun i => match sem map i with
                              | Some y => if p y then Some y else None
                              | None => None
                               end)  /\
-    Desc' m2 lb ub (fun i => match sem m2 i with
+    Desc' m2 lb ub (fun i => match sem map i with
                              | Some y => if p y then None else Some y
                              | None => None
                              end) ->
@@ -5792,6 +5769,955 @@ Proof.
   * simpl. repeat destruct_match; reflexivity.
 Qed.
 
+(*The following theorems are the axioms from ContainerAxioms and have no clear analogue in SetProofs*)
+
+(*Simpler definition of lookup*)
+Fixpoint lookup' (key : e) (map : Map e a) : option a :=
+  match map with
+  | Tip => None
+  | Bin sz k1 v1 lt rt => match compare key k1 with
+                          | Eq => Some v1 
+                          | Lt => lookup' key lt 
+                          | Gt => lookup' key rt
+                          end
+ end.  
+
+(*Prove the two definitions are equivalent*)
+Lemma lookup_lookup'_equiv : forall  (key : e) (map : Map e a),
+    lookup key map = lookup' key map.
+Proof.
+  intros. induction map.
+  - simpl. destruct (compare key k); try (reflexivity); assumption.
+  - simpl. reflexivity.
+Qed.  
+
+(*This lemma says that if two keys are equal, then the result of member is the same when either is called*)
+Lemma member_eq: forall {a : Type} (n : e) (n' : e) (m : Map e a),
+  n == n' = true ->
+  member n m = member n' m.
+Proof.
+  intros. 
+ induction m.
+   - simpl. destruct (compare n k) eqn : E.
+    + rewrite Ord_compare_Eq in E.  
+      apply Lemmas.Eq_trans_l  with(z:=k) in H.
+      rewrite E in H. symmetry in H. rewrite <- Ord_compare_Eq in H.
+      rewrite H. reflexivity.
+    + rewrite Ord_compare_Lt in E. 
+      apply Lemmas.Eq_le_r with(z:=k) in H. rewrite E in H. 
+      symmetry in H. rewrite <- Ord_compare_Lt in H. 
+      rewrite H. assumption.
+    + rewrite Ord_compare_Gt in E. apply Lemmas.Eq_le_l with (z:=k) in H.
+      rewrite E in H. symmetry in H. rewrite <- Ord_compare_Gt in H.
+      rewrite H. assumption.
+  - simpl. reflexivity.
+Qed.
+
+(*If we insert a (key, value) in a map, then looking up the key gives the value*)
+Lemma lookup_insert : forall `{Eq_ a} `{EqLaws a} (key: e) (value : a) (map : Map e a) lb ub,
+  Bounded map lb ub ->
+  isLB lb key = true ->
+  isUB ub key = true ->
+  lookup key (insert key value map)  == Some value = true.
+Proof.
+  intros. applyDesc insert_Desc. erewrite lookup_spec. specialize (Hsem key). 
+  rewrite Eq_Reflexive in Hsem. simpl in Hsem.
+  rewrite Hsem. apply Eq_Reflexive. apply HB.
+Qed. 
+
+(*If we lookup a key key1, the result is the same regardless of whether or not we have inserted key2 
+(a different key than key1)*)
+Lemma lookup_insert_neq : forall `{Eq_ a} `{EqLaws a} (key1: e) (key2: e) (value : a) (map : Map e a) lb ub,
+  Bounded map lb ub ->
+  isLB lb key2 = true ->
+  isUB ub key2 = true ->
+  key1 == key2 = false -> 
+  lookup key1 (insert key2 value map) = lookup key1 map.
+Proof.
+  intros. applyDesc insert_Desc. specialize (Hsem key1). rewrite H5 in Hsem.
+  simpl in Hsem. erewrite lookup_spec.  erewrite lookup_spec. apply Hsem. apply H2. apply HB.
+Qed.
+ 
+(*States that if we check for key1 in the map in which we have inserted key2, then either
+key1 was already in the map, or key1 == key2*)
+Lemma member_insert: forall key1 key2 value (map: Map e a) lb ub,
+  Bounded map lb ub ->
+  isLB lb key2 = true ->
+  isUB ub key2 = true ->
+  member key1 (insert key2 value map) = (key1 == key2) || member key1 map. 
+Proof.
+  intros. applyDesc insert_Desc. destruct (member key1 s) eqn : ?.
+  - erewrite member_spec in Heqb. destruct Heqb. specialize (Hsem key1). destruct (key1 == key2).
+    reflexivity. simpl in Hsem. simpl. symmetry. erewrite member_spec. exists x.
+    rewrite <- Hsem. assumption. apply H. apply HB.
+  - specialize (Hsem key1). destruct (key1 == key2). simpl in Hsem. 
+    assert (member key1 s = true). { erewrite member_spec. exists value. assumption. apply HB. }
+    rewrite Heqb in H2. inversion H2. simpl. simpl in Hsem.
+    assert (sem s key1 = None). { erewrite <- notMember_spec. unfold notMember. rewrite negb_true_iff.
+    assumption. apply HB. } rewrite Hsem in H2. erewrite <- notMember_spec in H2.
+    unfold notMember in H2. rewrite negb_true_iff in H2. symmetry. assumption. apply H.
+Qed. 
+
+(*If we lookup a key that is deleted, we should get None*)
+Lemma delete_eq : forall key (map : Map e a) lb ub,
+  Bounded map lb ub ->
+  lookup key (delete key map) = None.
+Proof.
+  intros. applyDesc delete_Desc. specialize (Hsem key). rewrite Eq_Reflexive in Hsem. rewrite <- Hsem.
+  eapply lookup_spec. apply HB.
+Qed.
+
+(*If we delete a key key2 and then lookup a different key key1, then it should be the same regardless of
+whether or not key2 was deleted.*)
+Lemma delete_neq : forall key1 key2 (map : Map e a) lb ub,
+  Bounded map lb ub ->
+  key1 == key2 = false ->
+  lookup key1 (delete key2 map) = lookup key1 map.
+Proof.
+  intros. applyDesc delete_Desc. erewrite lookup_spec. erewrite lookup_spec. 
+  specialize (Hsem key1). rewrite H0 in Hsem. assumption. apply H. apply HB.
+Qed.
+
+(*Same as above but for member*)
+Lemma member_delete_neq: forall key1 key2 (map: Map e a) lb ub,
+  Bounded map lb ub ->
+  key1 == key2 = false ->
+  member key2 (delete key1 map) = member key2 map.
+Proof.
+  intros. applyDesc delete_Desc. specialize (Hsem key2).
+  assert (key2 == key1 = false) by (order e). rewrite H1 in Hsem. destruct (member key2 s) eqn : ?.
+  - erewrite member_spec in Heqb. destruct Heqb. rewrite H2 in Hsem. symmetry. erewrite member_spec.
+    exists x. symmetry in Hsem. assumption. apply H. apply HB.
+  - assert (notMember key2 s = true). { unfold notMember. apply negb_true_iff. assumption. }
+    erewrite notMember_spec in H2. rewrite H2 in Hsem. symmetry in Hsem. erewrite <- notMember_spec in Hsem.
+    unfold notMember in Hsem. rewrite negb_true_iff in Hsem. symmetry. assumption. apply H. apply HB.
+Qed.
+
+(*States that if a key is not in the map, then looking it up will give None, and vice versa. *)
+Lemma non_member_lookup :
+  forall key (map: Map e a) lb ub,
+  Bounded map lb ub ->
+  (member key map = false) <-> (lookup key map = None).
+Proof.
+  intros. assert (notMember key map = true <-> member key map = false). { unfold notMember.
+  rewrite negb_true_iff. reflexivity. } rewrite <- H0. erewrite lookup_spec.
+  eapply notMember_spec. apply H. apply H.
+Qed.
+
+(*If two keys are equal (according to the Eq typeclass), then their values in 
+a map are equal*)
+Lemma lookup_eq : forall k k' (m : Map e a),
+    k == k' = true ->
+    lookup k m = lookup k' m.
+Proof.
+  intros. 
+ induction m.
+  - simpl. destruct (compare k k0) eqn : E.
+    + assert (compare k' k0 = Eq) by (order e). rewrite H0. reflexivity.
+    + assert (compare k' k0 = Lt) by (order e). rewrite H0. assumption.
+    + assert (compare k' k0 = Gt) by (order e). rewrite H0. assumption.
+  - reflexivity.
+Qed.
+
+(*This follows almost immediately from member_spec*)
+Lemma member_lookup : 
+  forall key (map: Map e a) lb ub,
+  Bounded map lb ub -> 
+  (member key map = true) <-> (exists value, lookup key map = Some value).
+Proof.
+  intros. assert(A:=H). eapply member_spec in A. eapply lookup_spec in H.
+  rewrite <- H in A. apply A.
+Qed. 
+
+(** ** Verification of [null] *)
+Lemma null_empty: 
+    @null e a empty = true.
+Proof.
+  unfold null. simpl. reflexivity.
+Qed. 
+
+(*A key is a member of the union of two maps whenever it is a member of at least one of the maps*)
+Lemma member_union :
+  forall key (map1: Map e a) map2 lb ub,
+  Bounded map1 lb ub ->
+  Bounded map2 lb ub ->
+  member key (union map1 map2) = member key map2 || member key map1.
+Proof.
+  intros. applyDesc union_Desc. specialize (Hsem key). destruct (member key s) eqn : ?.
+  - erewrite member_spec in Heqb. destruct Heqb. rewrite H1 in Hsem. destruct (sem map1 key) eqn : ?.
+    inversion Hsem; subst. assert (member key map1 = true). { erewrite member_spec.
+    exists a0. assumption. apply H. } rewrite H2. rewrite orb_true_r. reflexivity.
+    simpl in Hsem. assert (member key map2 = true). { erewrite member_spec. exists x. symmetry.
+    assumption. apply H0. } rewrite H2. reflexivity. apply HB.
+  - rewrite <- negb_true_iff in Heqb. assert (notMember key s = true). { unfold notMember.
+    assumption. } eapply notMember_spec in H1. rewrite H1 in Hsem. destruct (sem map1 key) eqn : ?.
+    inversion Hsem. destruct (sem map2 key) eqn : ?. inversion Hsem. 
+    erewrite <- notMember_spec in Heqo. erewrite <- notMember_spec in Heqo0.
+    unfold notMember in *. rewrite negb_true_iff in *. rewrite Heqo. rewrite Heqo0. reflexivity.
+    apply H0. apply H. apply HB.
+Qed.
+
+(*The union of a map with the empty map (in both directions) is itself*)
+Lemma union_nil_l : forall (map: Map e a) ub lb,
+  Bounded map ub lb ->
+  union empty map = map.
+Proof.
+  intros. unfold empty. induction H.
+  - reflexivity.
+  - simpl. destruct s1 eqn : ?. reflexivity. destruct s2 eqn : ?. reflexivity.
+    unfold insertR. unfold singleton. rewrite H3. simpl. reflexivity.
+Qed.
+
+Lemma union_nil_r : forall (map: Map e a) ub lb,
+  Bounded map ub lb ->
+  union map empty = map.
+Proof.
+  intros. induction H.
+  - simpl. reflexivity.
+  - simpl. destruct s1. reflexivity. destruct s2. reflexivity. reflexivity.
+Qed.
+
+(*The difference between a map and itself is the empty map*)
+Lemma difference_self: forall (map: Map e a) lb ub,
+  Bounded map lb ub ->
+  difference map map = empty.
+Proof.
+  intros. 
+ eapply difference_Desc. apply H. apply H. intros.
+  unfold diffo in H3.
+  assert (forall i, sem s i = None). { intros i. specialize (H3 i).
+  destruct (sem map i); assumption. } apply empty_no_elts. apply H4.
+Qed. 
+
+(*The difference of a map with the empty map is itself*)
+Lemma difference_nil_r: forall `{Eq_ a} `{EqLaws a} (B : Type) (map: Map e a) lb ub,
+  Bounded map lb ub ->
+  difference map (@empty e B) = map.
+Proof.
+  intros. inversion H2.
+  - simpl. reflexivity.
+  - simpl. reflexivity.
+Qed.
+
+(*The difference of the empty map with any map is empty*)
+Lemma difference_nil_l: forall `{Eq_ a} `{EqLaws a} (B : Type) (map: Map e a) lb ub (key : e),
+  Bounded map lb ub ->
+  difference (@empty e B) map = empty.
+Proof.
+  intros. inversion H2.
+  - simpl. reflexivity.
+  - simpl. unfold empty. reflexivity.
+Qed.
+
+(*Follows from sem_inside, says that if a key is in a map, it is between the bounds*)
+Lemma keys_inside_bounds : forall (map: Map e a) key lb ub,
+  Bounded map lb ub ->
+  member key map = true ->
+  isLB lb key = true /\ isUB ub key = true .
+Proof.
+  intros. eapply member_spec in H0. destruct H0.
+  eapply sem_inside. apply H. apply H0. apply H.
+Qed.
+
+(*If a key is in a map, the difference of the singleton map containing only that key
+and the original map is empty*)
+Lemma difference_Tip_member: forall (map: Map e a) (key :e) lb ub,
+  Bounded map lb ub ->
+  member key map = true ->
+  forall (value : a), difference (singleton key value) map = empty.
+Proof.
+  intros. assert (A:=H0). apply (keys_inside_bounds _ _ lb ub) in H0. destruct H0.
+  applyDesc singleton_Desc. eapply difference_Desc. apply HB. apply H. intros.
+  eapply empty_no_elts. intros. specialize (H5 i). specialize (Hsem i).
+  destruct (i == key) eqn : ?. simpl in Hsem. rewrite Hsem in H5.
+  erewrite member_spec in A. destruct A. erewrite sem_resp_eq in H6.
+  rewrite H6 in H5. simpl in H5. assumption. order e. apply H. simpl in Hsem.
+  rewrite Hsem in H5. destruct (sem map i); simpl in H5; assumption. apply H.
+Qed.
+
+
+(*We cannot use Coq equality because even though the structure of a singleton tree is unique, 
+it k1 == k2, singleton k1 v == singleton k2 v, and both are characterized by
+[forall i, sem m i = SomeIf (i == k1) v]*)
+Lemma difference_Tip_non_member: forall `{EqLaws a} (map: Map e a) (key :e) lb ub,
+  Bounded map lb ub ->
+  isUB ub key = true ->
+  isLB lb key = true ->
+  member key map = false ->
+  forall (value : a), difference (singleton key value) map == (singleton key value) = true.
+Proof.
+  intros. assert (Bounded (singleton key value) lb ub). apply BoundedBin; try (apply BoundedTip); try(assumption).
+  simpl. reflexivity. simpl. unfold balance_prop. simpl. omega. eapply difference_Desc.
+  - apply H5.
+  - apply H1.
+  - intros. unfold diffo in H9.
+    assert( forall i : e, sem s i = SomeIf(i == key) value). { intros. specialize (H9 i).
+    destruct (i == key) eqn : ?. assert (sem map i = sem map key) by (apply sem_resp_eq; assumption).
+    rewrite H10 in H9. assert (sem map key = None). eapply notMember_spec.
+    apply H1. unfold notMember. rewrite negb_true_iff. assumption. rewrite H11 in H9.
+    unfold SomeIf. rewrite H9. rewrite (sem_resp_eq _ i key). simpl. rewrite Eq_Reflexive.
+    simpl. reflexivity. apply Heqb. simpl. destruct(sem map i) eqn : ?.
+    assumption. simpl in H9. rewrite Heqb in H9. simpl in H9. assumption. }
+    applyDesc singleton_Desc. eapply weak_equals_spec. apply H6. apply HB.
+    intros. specialize (H10 i). specialize (Hsem i). rewrite H10. rewrite Hsem.
+    apply Eq_Reflexive.
+Qed.
+
+(*Function that represents sem on a filtered list. It is much easier to work with and helps prove
+the next few lemmas about how filter behaves on maps. Unfortunately filterWithKey_Desc is not enough, 
+since most of these have a claim about filter in the hypothesis*)
+Fixpoint sem_filter (m: Map e a) f i:=
+  match m with
+  |Tip => None
+  |Bin _ k v m1 m2 => match compare i k with
+                     | Lt => sem_filter m1 f i
+                     | Eq => SomeIf (f k v) v
+                     | Gt => sem_filter m2 f i
+                    end
+  end.
+
+(*Proves the equivalence of this function with using sem on the filtered map directly*)
+Lemma sem_filter_equiv: forall m lb ub key f,
+  Bounded m lb ub ->
+  Proper ((fun (i j : e) => _GHC.Base.==_ i j = true) ==> eq) f ->
+  sem (filterWithKey f m) key = sem_filter m f key.
+Proof.
+  intros. induction H.
+  - simpl. reflexivity.
+  - eapply filterWithKey_Desc. apply BoundedBin. apply H. apply H1. apply H2. apply H3.
+    apply H4. apply H5. apply H0. intros. simpl in *. specialize (H8 key).
+    destruct (compare key x) eqn : ?.
+    + assert (key == x = true) by (order e). rewrite H9 in H8.
+      assert (sem s1 key = None). eapply sem_outside_above. apply H. solve_Bounds. rewrite H10 in H8.
+      simpl in H8. unfold SomeIf. assert (f x v = f key v). apply equal_f. apply H0. order e.
+      rewrite H11. assumption.
+    + rewrite <- IHBounded1. eapply filterWithKey_Desc. apply H. apply H0. intros.
+      specialize (H11 key). destruct (sem s1 key) eqn : ?. simpl in H8.
+      rewrite <- H8 in H11. symmetry. assumption.
+      assert (key == x = false) by (order e). rewrite H12 in H8. assert (sem s2 key = None).
+      eapply sem_outside_below. apply H1. solve_Bounds. rewrite H13 in H8. simpl in H8.
+      rewrite H8. symmetry. assumption.
+    + assert (sem s1 key = None). eapply sem_outside_above. apply H. solve_Bounds. rewrite H9 in H8.
+      simpl in H8. assert (key == x = false) by (order e). rewrite H10 in H8; simpl in H8.
+      rewrite <- IHBounded2. eapply filterWithKey_Desc. apply H1. apply H0. intros.
+      specialize (H13 key). rewrite <- H13 in H8. apply H8.
+Qed.
+
+(*If a key, value pair is in the filtered map, it was in the original map*)
+Lemma filterPreservesValues: forall m lb ub f,
+  Bounded m lb ub ->
+  Proper ((fun (i j : e) => _GHC.Base.==_ i j = true) ==> eq) f ->
+  forall i v, sem (filterWithKey f m) i = Some v -> sem m i = Some v.
+Proof.
+  intros. rewrite (sem_filter_equiv m lb ub i f H) in H1. induction H.
+  - simpl in H1. inversion H1.
+  - simpl in H1. simpl. destruct (compare i x) eqn : ?.
+    + assert (i == x = true) by (order e). rewrite H7. simpl. assert (sem s1 i = None).
+      eapply sem_outside_above. apply H. solve_Bounds. rewrite H8. unfold SomeIf in H1. simpl.
+      destruct (f x v0). assumption. inversion H1.
+    + apply IHBounded1 in H1. rewrite H1. reflexivity.
+    + assert (sem s1 i = None). eapply sem_outside_above. apply H. solve_Bounds. rewrite H7.
+      assert (i == x = false) by (order e). rewrite H8. simpl. apply IHBounded2.
+      assumption.
+  - assumption.
+Qed.
+
+(*If a key, value pair is in the filtered map, the function returns true on the pair*)
+Lemma filter_sem_true: forall m lb ub f,
+  Bounded m lb ub ->
+  Proper ((fun (i j : e) => _GHC.Base.==_ i j = true) ==> eq) f ->
+  forall i v, sem (filterWithKey f m) i = Some v -> f i v = true.
+Proof.
+  intros. rewrite (sem_filter_equiv _ lb ub) in H1. induction H.
+  - simpl in H1. inversion H1.
+  - simpl in H1. destruct (compare i x) eqn : ?.
+    + unfold SomeIf in H1. destruct (f x v0) eqn : ?. 
+      rewrite <- Heqb. inversion H1; subst. eapply equal_f. apply H0. order e. inversion H1.
+    + apply IHBounded1. apply H1.
+    + apply IHBounded2. apply H1.
+  - assumption.
+  - assumption.
+Qed.
+
+(*Conversely, if a key, value pair was in the map and not in the filtered map, f k v is false*)
+Lemma filter_sem_false: forall m lb ub f,
+  Bounded m lb ub ->
+  Proper ((fun (i j : e) => _GHC.Base.==_ i j = true) ==> eq) f ->
+  forall i v, sem m i = Some v ->
+   sem (filterWithKey f m) i = None -> f i v = false.
+Proof.
+  intros. rewrite (sem_filter_equiv _ lb ub) in H2. induction H.
+  - simpl in H1. inversion H1.
+  - simpl in H2. destruct (compare i x) eqn : ?.
+    + unfold SomeIf in H2. destruct (f x v0) eqn : ?. inversion H2. 
+      rewrite <- Heqb. simpl in H1. assert (sem s1 i = None). { eapply sem_outside_above. apply H.
+      solve_Bounds. } rewrite H8 in H1. simpl in H1. assert (i == x = true) by (order e).
+      rewrite H9 in H1. inversion H1; subst. eapply equal_f. apply H0. assumption. 
+    + simpl in H1. destruct (sem s1 i) eqn : ?. inversion H1; subst. apply IHBounded1.
+      reflexivity. assumption. assert (i == x = false) by (order e). assert (sem s2 i = None). {
+      eapply sem_outside_below. apply H3. solve_Bounds. } rewrite H8 in H1. rewrite H9 in H1.
+      inversion H1.
+    + simpl in H1. assert (sem s1 i = None). { eapply sem_outside_above. apply H. solve_Bounds. }
+      assert (i == x = false) by (order e). rewrite H8 in H1. rewrite H9 in H1. simpl in H1.
+      apply IHBounded2. assumption. assumption.
+  - assumption.
+  - assumption.
+Qed.
+
+(*Note: needed to add assumption that f, f', and f && f'respect equality - the last to avoid
+using functional extensionality*)
+Lemma filterWithKey_comp: forall `{EqLaws a} f f' (m: Map e a) lb ub ,
+  Bounded m lb ub ->
+  Proper ((fun (i j : e) => _GHC.Base.==_ i j = true) ==> eq) f ->
+  Proper ((fun i j : e => _GHC.Base.==_ i j = true) ==> eq) f' ->
+  Proper ((fun i j : e => _GHC.Base.==_ i j = true) ==> eq) (fun v a => f v a && f' v a) ->
+  filterWithKey f (filterWithKey f' m) == filterWithKey (fun v a => f v a && f' v a) m = true.
+Proof.
+  intros. assert (Bounded (filterWithKey f' m) lb ub). apply filterWithKey_Bounded. apply H1.
+  eapply filterWithKey_Desc. apply H5. apply H2. intros.
+  eapply filterWithKey_Desc. apply H1. apply H4. 
+  intros.
+  - eapply weak_equals_spec. apply H6. apply H9. intros.
+    destruct (sem (filterWithKey f' m) i) eqn : ?. 
+    + specialize (H8 i). rewrite Heqo in H8.
+      assert (A:= Heqo). eapply filter_sem_true in Heqo. eapply filterPreservesValues in A.
+      specialize (H11 i). rewrite A in H11. rewrite Heqo in H11. rewrite andb_true_r in H11.
+      rewrite H11. rewrite H8. apply Eq_Reflexive. apply H1. apply H3. apply H1. apply H3.
+    + specialize (H8 i). rewrite Heqo in H8. specialize (H11 i). destruct (sem m i) eqn : ?.
+      assert (f' i a0 = false). { eapply filter_sem_false. apply H1. apply H3. apply Heqo0.
+      apply Heqo. } rewrite H12 in H11. rewrite andb_false_r in H11. rewrite H11. rewrite H8.
+      apply Eq_Reflexive. rewrite H8. rewrite H11. apply Eq_Reflexive.
+Qed.  
+
+Lemma filter_comp: forall `{EqLaws a} (f: a -> bool) (f': a -> bool) (m: Map e a) lb ub ,
+  Bounded m lb ub ->
+  Internal.filter f (Internal.filter f' m) == Internal.filter (fun v => f v && f' v) m = true.  
+Proof.
+  intros. unfold filter. eapply filterWithKey_comp. apply H1. unfold respectful.
+  unfold Proper. intros. reflexivity. unfold respectful. unfold Proper.
+  intros. reflexivity.
+  - unfold respectful. unfold Proper. intros. reflexivity.
+Qed.
+
+(*This is FALSE as long as the type a is inhabited by at >= 2 nonequal elements*)
+Lemma filterWithKey_insert_false:forall `{EqLaws a} (key: e) (v v1: a), v == v1 = false -> 
+~(forall  key v lb ub f m,
+  Bounded m lb ub ->
+  isUB ub key = true ->
+  isLB lb key = true ->
+  Proper ((fun (i j : e) => _GHC.Base.==_ i j = true) ==> eq) f ->
+  filterWithKey f (insert key v m) ==
+  (if (f key v) then
+    insert key v (filterWithKey f m)
+    else filterWithKey f m) = true).
+Proof.
+  intros. intro contra. remember (singleton key v1) as m1. remember (fun (x : e) value => value == v1) as f1.
+  assert (_GHC.Base.==_ (filterWithKey f1 (insert key v m1))
+           (if f1 key v then insert key v (filterWithKey f1 m1) else filterWithKey f1 m1) = true).
+  apply (contra _ _ None None).  rewrite Heqm1. unfold singleton. apply BoundedBin.
+  apply BoundedTip. apply BoundedTip. solve_Bounds. solve_Bounds. simpl. reflexivity. simpl.
+  unfold balance_prop. omega. solve_Bounds. solve_Bounds. rewrite Heqf1. unfold respectful.
+  unfold Proper. intros. reflexivity.
+  rewrite Heqm1 in H2. rewrite weak_equals_spec in H2. specialize (H2 key).
+  erewrite sem_filter_equiv in H2. unfold singleton in H2. unfold insert at 1 in H2.
+  assert (compare key key = Eq) by (order e). rewrite H3 in H2.
+  assert (PtrEquality.ptrEq v v1 = false). { destruct (PtrEquality.ptrEq v v1) eqn : ?.
+  apply PtrEquality.ptrEq_eq in Heqb. subst. rewrite Eq_Reflexive in H1. inversion H1. reflexivity. }
+  rewrite H4 in H2. rewrite andb_false_l in H2. assert (f1 key v = false). { rewrite Heqf1. order a. }
+  simpl in H2. rewrite H5 in H2. rewrite H3 in H2. simpl in H2.
+  assert (f1 key v1 = true). { rewrite Heqf1.  order a. } rewrite H6 in H2.
+  destruct (PtrEquality.ptrEq Tip Tip). simpl in H2. rewrite Eq_Reflexive in H2. simpl in H2.
+  inversion H2. simpl in H2. rewrite Eq_Reflexive in H2. simpl in H2. inversion H2.
+  apply insert_WF. unfold WF. unfold singleton. apply BoundedBin. apply BoundedTip. apply BoundedTip.
+  solve_Bounds. solve_Bounds. simpl. reflexivity. unfold balance_prop. simpl. omega. 
+  unfold respectful. unfold Proper. intros. rewrite Heqf1. reflexivity. apply filterWithKey_Bounded.
+  apply insert_WF. applyDesc singleton_Desc. assert (isLB None key = true) by (solve_Bounds).
+  apply H3. assert (isUB None key = true) by (solve_Bounds). apply H3. apply HB.
+  destruct (f1 key v). applyDesc singleton_Desc. assert (isLB None key = true) by (solve_Bounds).
+  apply H3. assert (isUB None key = true) by (solve_Bounds). apply H3. 
+  apply insert_WF. apply filterWithKey_Bounded. assumption. applyDesc singleton_Desc.
+   assert (isLB None key = true) by (solve_Bounds).
+  apply H3. assert (isUB None key = true) by (solve_Bounds). apply H3. apply filterWithKey_Bounded.
+  assumption.
+Qed.
+
+Lemma lookup_filterWithKey:
+  forall key value (m: Map e a) f lb ub,
+  Bounded m lb ub ->
+  Proper ((fun (i j : e) => _GHC.Base.==_ i j = true) ==> eq) f ->
+  lookup key (filterWithKey f m) = Some value ->
+  lookup key m = Some value.
+Proof.
+  intros. erewrite lookup_spec in H1. eapply filterPreservesValues in H1.
+  erewrite lookup_spec. assumption. eassumption. eassumption. eassumption.
+  apply filterWithKey_Bounded. eassumption.
+Qed.
+
+(*Have to add {EqLaws a} due to comparing maps for equality*)
+Lemma filter_true: forall `{EqLaws a} (m: Map e a) lb ub,
+  Bounded m lb ub ->
+  filter (const true) m == m = true.
+Proof.
+  intros. unfold filter. eapply filterWithKey_Desc. eassumption.
+  unfold respectful. unfold Proper. intros. reflexivity. intros.
+  eapply weak_equals_spec; try(eassumption). intros.
+  simpl in H4. specialize (H4 i). destruct (sem s i). destruct (sem m i).
+  inversion H4; subst; apply Eq_Reflexive. inversion H4. destruct (sem m i).
+  inversion H4. apply Eq_Reflexive.
+Qed.
+
+
+Definition sem_intersect (m1: Map e a)(m2: Map e a) i :=
+  match (sem m1 i), (sem m2 i) with
+  | Some v, Some v2 => Some v
+  | _, _ => None
+  end.
+
+Lemma sem_intersect_equiv: forall m1 m2 lb ub key,
+  Bounded m1 lb ub ->
+  Bounded m2 lb ub ->
+  sem (intersection m1 m2) key = sem_intersect m1 m2 key.
+Proof.
+  intros. applyDesc intersection_Desc. specialize (Hsem key).
+  destruct (sem m1 key ) eqn : ?. destruct (sem m2 key) eqn: ?.
+  simpl in Hsem. unfold sem_intersect. rewrite Heqo. rewrite Heqo0. assumption.
+  simpl in Hsem. unfold sem_intersect. rewrite Heqo. rewrite Heqo0. assumption.
+  unfold sem_intersect. rewrite Heqo. destruct (sem m2 key); simpl in Hsem; assumption.
+Qed.
+
+Lemma lookup_intersection: forall v1 key m1 m2 lb ub,
+  Bounded m1 lb ub ->
+  Bounded m2 lb ub ->
+  lookup key m1 = Some v1 /\ (exists v2, lookup key m2 = Some v2) <->
+  lookup key (intersection m1 m2) = Some v1.
+Proof.
+  intros. split; intros.
+  - applyDesc intersection_Desc. erewrite lookup_spec. destruct H1.
+    rewrite (lookup_spec H) in H1. specialize (Hsem key). rewrite H1 in Hsem.
+    destruct H2. rewrite (lookup_spec H0) in H2. rewrite H2 in Hsem. simpl in Hsem.
+    assumption. eassumption.
+  - erewrite lookup_spec in H1. erewrite sem_intersect_equiv in H1.
+    unfold sem_intersect in H1. destruct (sem m1 key) eqn : ?.
+    destruct (sem m2 key) eqn : ?. inversion H1; subst.
+    split. erewrite lookup_spec. assumption. eassumption. exists a1.
+    erewrite lookup_spec. assumption. eassumption. inversion H1. inversion H1.
+    eassumption. eassumption. applyDesc intersection_Desc. apply HB.
+Qed.
+
+Definition sem_union (m1: Map e a)(m2: Map e a) i :=
+  match (sem m1 i), (sem m2 i) with
+  | Some v, _ => Some v
+  | _, Some v2 => Some v2
+  | _, _ => None
+  end.
+
+Lemma sem_union_equiv: forall m1 m2 lb ub key,
+  Bounded m1 lb ub ->
+  Bounded m2 lb ub ->
+  sem (union m1 m2) key = sem_union m1 m2 key.
+Proof.
+  intros. applyDesc union_Desc. specialize (Hsem key). unfold sem_union.
+  destruct (sem m1 key) eqn : ?. destruct (sem m2 key) eqn : ?.
+  - simpl in Hsem. assumption.
+  - rewrite oro_None_r in Hsem. assumption.
+  - simpl in Hsem. rewrite Hsem. destruct (sem m2 key); reflexivity.
+Qed.
+
+Lemma lookup_union:
+  forall key value (m1: Map e a) m2 lb ub,
+  Bounded m1 lb ub ->
+  Bounded m2 lb ub ->
+  lookup key m1 = Some value \/ (lookup key m1 = None /\ lookup key m2 = Some value) <->
+  lookup key (union m1 m2) = Some value.
+Proof.
+  intros. split; intros. 
+  - applyDesc union_Desc. erewrite lookup_spec. specialize (Hsem key). destruct H1.
+    rewrite (lookup_spec H) in H1. rewrite H1 in Hsem. simpl in Hsem. assumption.
+    destruct H1. rewrite (lookup_spec H) in H1. rewrite (lookup_spec H0) in H2.
+    rewrite H1 in Hsem. rewrite H2 in Hsem. simpl in Hsem. assumption. apply HB.
+  - erewrite lookup_spec in H1. erewrite sem_union_equiv in H1. unfold sem_union in H1.
+    destruct (sem m1 key) eqn : ?.
+    + left. rewrite (lookup_spec H). inversion H1; subst; assumption.
+    + destruct (sem m2 key) eqn : ?. right. split. rewrite (lookup_spec H).
+      assumption. rewrite (lookup_spec H0). inversion H1; subst; assumption. inversion H1.
+   + apply H.
+   + apply H0.
+    + applyDesc union_Desc. apply HB.
+Qed.
+
+
+(*Lemma partition_preserves_values: forall m P key value lb ub,
+  Bounded m lb ub ->
+  Proper ((fun (i j : e) => _GHC.Base.==_ i j = true) ==> eq) P ->
+  sem m key = Some value ->
+  P key value = true ->
+  sem (fst (partitionWithKey P m)) key = Some value.
+Proof.
+  intros. induction H.
+  - simpl. simpl in H1. inversion H1.
+  - eapply (partitionWithKey_spec _ _ lb ub). apply BoundedBin; assumption. assumption. intros.
+    simpl. apply H8. intros. specialize (H11 key).  simpl.
+
+
+ eapply  split; split; intros.
+  - pose proof partitionWithKey_spec. 
+    specialize (H3 P m lb ub H H0 (fun m => fst m (partitionWithKey P m)) key = Some value). simpl in H2.*)
+
+
+Lemma fst_partition_sem: forall m P key lb ub,
+  Bounded m lb ub ->
+  Proper ((fun (i j : e) => _GHC.Base.==_ i j = true) ==> eq) P ->
+  sem (fst (partitionWithKey P m)) key = sem_filter m P key.
+Proof.
+  intros. induction H.
+  - reflexivity.
+  - apply (partitionWithKey_spec _ _ lb ub).
+    + apply BoundedBin; assumption.
+    + assumption.
+    + intros. simpl. simpl in H6. apply H6. intros. destruct (compare key x) eqn : ?.
+      * specialize (H9 key). assert (sem s1 key = None). eapply sem_outside_above. apply H.
+        solve_Bounds. rewrite H10 in H9. simpl in H9. assert (key == x = true) by (order e).
+        rewrite H11 in H9. simpl in H9. unfold SomeIf. assert (P key v = P x v).
+        apply equal_f. apply H0. apply H11. rewrite <- H12. apply H9.
+      * rewrite <- IHBounded1. eapply partitionWithKey_spec. apply H. apply H0. intros.
+        simpl. apply H10. intros. specialize (H13 key). specialize (H9 key).
+        destruct (sem s1 key) eqn : ?. simpl in H9.
+        rewrite H9. rewrite H13. reflexivity. assert (key == x = false) by (order e).
+        assert (sem s2 key = None). eapply sem_outside_below. apply H1. solve_Bounds. 
+        rewrite H14 in H9. rewrite H15 in H9. simpl in H9. rewrite H9. rewrite H13.
+        reflexivity.
+      * rewrite <- IHBounded2. eapply partitionWithKey_spec. apply H1. apply H0. intros.
+        simpl. apply H10. intros. specialize (H13 key). specialize (H9 key).
+        assert (sem s1 key = None). eapply sem_outside_above. apply H. solve_Bounds.
+        assert (key == x = false) by (order e). rewrite H14 in H9. rewrite H15 in H9.
+        simpl in H9. rewrite H13. rewrite H9. reflexivity.
+Qed.
+
+Lemma snd_partition_sem: forall m P key lb ub,
+  Bounded m lb ub ->
+  Proper ((fun (i j : e) => _GHC.Base.==_ i j = true) ==> eq) P ->
+  sem (snd (partitionWithKey P m)) key = sem_filter m (fun a b => negb( P a b)) key.
+Proof.
+  intros. induction H.
+  - reflexivity.
+  - apply (partitionWithKey_spec _ _ lb ub).
+    + apply BoundedBin; assumption.
+    + assumption.
+    + intros. simpl. simpl in H6. apply H6. intros. destruct (compare key x) eqn : ?.
+      * specialize (H9 key). assert (sem s1 key = None). eapply sem_outside_above. apply H.
+        solve_Bounds. rewrite H10 in H9. simpl in H9. assert (key == x = true) by (order e).
+        rewrite H11 in H9. simpl in H9. unfold SomeIf. assert (P key v = P x v).
+        apply equal_f. apply H0. apply H11. rewrite <- H12. destruct (P key v) eqn : ?;
+        simpl; apply H9.
+      * rewrite <- IHBounded1. eapply partitionWithKey_spec. apply H. apply H0. intros.
+        simpl. apply H10. intros. specialize (H13 key). specialize (H9 key).
+        destruct (sem s1 key) eqn : ?. simpl in H9.
+        rewrite H9. rewrite H13. reflexivity. assert (key == x = false) by (order e).
+        assert (sem s2 key = None). eapply sem_outside_below. apply H1. solve_Bounds. 
+        rewrite H14 in H9. rewrite H15 in H9. simpl in H9. rewrite H9. rewrite H13.
+        reflexivity.
+      * rewrite <- IHBounded2. eapply partitionWithKey_spec. apply H1. apply H0. intros.
+        simpl. apply H10. intros. specialize (H13 key). specialize (H9 key).
+        assert (sem s1 key = None). eapply sem_outside_above. apply H. solve_Bounds.
+        assert (key == x = false) by (order e). rewrite H14 in H9. rewrite H15 in H9.
+        simpl in H9. rewrite H13. rewrite H9. reflexivity.
+Qed.
+
+Lemma partitionPreservesNone: forall m lb ub f,
+  Bounded m lb ub ->
+  Proper ((fun (i j : e) => _GHC.Base.==_ i j = true) ==> eq) f ->
+  forall i, sem m i = None -> sem_filter m f i = None.
+Proof.
+  intros. induction H.
+  - reflexivity.
+  - simpl. simpl in H1. destruct (compare i x) eqn : ?.
+   + destruct (sem s1 i). inversion H1. assert (i == x = true) by (order e).
+    rewrite H7 in H1. simpl in H1. inversion H1.
+   + destruct (sem s1 i). inversion H1. destruct (i == x) eqn : ?.
+     inversion H1. order e.
+   + destruct (sem s1 i). inversion H1. destruct (i == x) eqn : ?. inversion H1.
+     destruct (sem s2 i) eqn : ?. inversion H1. apply IHBounded2. reflexivity.
+Qed.
+
+(*If a key, value pair is in the filtered map, it was in the original map*)
+Lemma partitionPreservesValues: forall `{EqLaws a} m lb ub f,
+  Bounded m lb ub ->
+  Proper ((fun (i j : e) => _GHC.Base.==_ i j = true) ==> eq) f ->
+  forall i v, sem_filter m f i == Some v = true -> sem m i == Some v = true.
+Proof.
+  intros. induction H1.
+  - simpl in H3. inversion H3.
+  - simpl. destruct (compare i x) eqn : ?.
+    + assert (sem s1 i = None). eapply sem_outside_above. apply H1_. solve_Bounds.
+      simpl in H3. rewrite Heqc in H3. rewrite H7. simpl. assert (i == x = true) by (order e).
+      rewrite H8. simpl. destruct (f x v0). simpl in H3. assumption. inversion H3.
+    + simpl in H3. rewrite Heqc in H3. destruct (sem s1 i) eqn : ?. simpl.
+      apply IHBounded1. apply H3. eapply partitionPreservesNone in Heqo.
+      rewrite Heqo in H3. inversion H3. apply H1_. apply H2.
+    + simpl in H3. rewrite Heqc in H3. assert (sem s1 i = None). eapply sem_outside_above.
+      apply H1_. solve_Bounds. rewrite H7. assert (i == x = false) by (order e). rewrite H8.
+      simpl. apply IHBounded2. apply H3.
+Qed.
+
+(*Note: had to change all to Haskell equality since that is the only information equality of maps
+gives us*)
+(*Also, unfortunately we need another extra hypothesis because of functional extensionality -
+that the negation of P is proper as well*)
+(*Also, I don't think this is actually true (the reverse direction) - it seems to
+say that if lookup key m == Some value = true, then for all maps m',
+we have the 3 conditions, which is not true
+TODO: ASk*)
+Lemma lookup_partition: forall key value `{EqLaws a} (m: Map e a) m' P lb ub,
+  Bounded m lb ub ->
+  Bounded m' lb ub ->
+  Proper ((fun (i j : e) => _GHC.Base.==_ i j = true) ==> eq) P ->
+  Proper ((fun (i j : e) => _GHC.Base.==_ i j = true) ==> eq) (fun a b => negb (P a b)) ->
+  ((m' == fst (partitionWithKey P m) = true) \/ (m' == snd (partitionWithKey P m) = true)) /\
+  lookup key m' == Some value = true -> lookup key m == Some value = true.
+Proof.
+  intros. 
+  - destruct H5. destruct H5.
+    + rewrite (weak_equals_spec m') in H5. specialize (H5 key).
+      erewrite fst_partition_sem in H5. erewrite lookup_spec.
+      erewrite lookup_spec in H6. assert ((sem_filter m P key) == (Some value) = true).
+      eapply Eq_Transitive. apply Eq_Symmetric. apply H5. apply H6. 
+      eapply partitionPreservesValues. apply H1. apply H3. apply H7. apply H2. apply H1.
+      apply H1. apply H3. apply H2. eapply partitionWithKey_spec. apply H1. apply H3.
+      intros. simpl. apply H7. intros. apply H8.
+    + rewrite weak_equals_spec in H5. specialize (H5 key).
+      erewrite snd_partition_sem in H5. erewrite lookup_spec. erewrite lookup_spec in H6.
+      assert (sem_filter m (fun a b => negb (P a b)) key == Some value = true). eapply Eq_Transitive.
+      apply Eq_Symmetric. apply H5. apply H6. eapply partitionPreservesValues. apply H1.
+      apply H4. apply H7. apply H2. apply H1. apply H1. apply H3. apply H2.
+      eapply partitionWithKey_spec. apply H1. apply H3. intros. simpl. apply H7.
+      intros. apply H8.
+Qed.
+
+Lemma sem_filter_in_map: forall key value map lb ub f,
+  Bounded map lb ub ->
+  Proper ((fun (i j : e) => _GHC.Base.==_ i j = true) ==> eq) f ->
+  sem map key = Some value ->
+  f key value = true ->
+  sem_filter map f key = Some value.
+Proof.
+  intros. induction H.  
+  - inversion H1.
+  - simpl. simpl in H1. destruct (compare key x) eqn : ?.
+     + assert (sem s1 key = None). eapply sem_outside_above. apply H. solve_Bounds.
+       rewrite H8 in H1. assert (key == x = true) by (order e). rewrite H9 in H1.
+        simpl in H1. inversion H1; subst. assert (f x value = f key value).
+        apply equal_f. apply H0. order e. rewrite H6.
+        rewrite H2. simpl. reflexivity.
+      + apply IHBounded1. destruct (sem s1 key). inversion H1; subst; reflexivity.
+        destruct (key == x) eqn : ?. order e. destruct (sem s2 key) eqn : ?. solve_Bounds.
+        inversion H1.
+      + apply IHBounded2. destruct (sem s1 key) eqn : ?. solve_Bounds. 
+        destruct (key == x) eqn : ?. order e. simpl in H1. apply H1.
+Qed. 
+
+Lemma eq_coq_implies_haskell : forall {a} `{EqLaws a} (x y : a),
+  x = y -> x == y = true.
+Proof.
+  intros. subst. apply Eq_Reflexive.
+Qed.
+
+(*Need to have proven EqLaws for Map first, since we need to show that left = snd Partition
+-> left == snd Partition, but we need equality in the hypothesis because equality of
+maps does not imply bounds at all*)
+Lemma lookup_partition': forall `{EqLaws a} key value map left right f lb ub,
+  Bounded map lb ub ->
+  Proper ((fun (i j : e) => _GHC.Base.==_ i j = true) ==> eq) f ->
+  Proper ((fun (i j : e) => _GHC.Base.==_ i j = true) ==> eq) (fun a b => negb (f a b)) ->
+  lookup key map = Some value ->
+  (left, right) = partitionWithKey f map  ->
+  lookup key left == Some value = true \/ lookup key right == Some value = true.
+Proof.
+  intros. assert (left = fst (partitionWithKey f map)). unfold fst. rewrite <- H5.
+  reflexivity. assert (right = snd (partitionWithKey f map)). unfold snd. rewrite <- H5.
+  reflexivity. assert (A :=H6). assert (A1:=H7).
+  assert(forall i, sem left i =  sem (fst (partitionWithKey f map)) i). intros. rewrite H6.
+  reflexivity. assert (forall i, sem right i = sem (snd (partitionWithKey f map)) i).
+  rewrite H7. intros. reflexivity.
+  erewrite lookup_spec in H4. erewrite lookup_spec. erewrite lookup_spec.
+  - specialize (H8 key). specialize (H9 key). erewrite fst_partition_sem in H8.
+    erewrite snd_partition_sem in H9. destruct (f key value) eqn : ?.
+    erewrite sem_filter_in_map in H8. rewrite H8. left. apply Eq_Reflexive.
+    apply H1. apply H2. apply H4. apply Heqb.
+    assert ((fun a b => negb (f a b)) key value = true). rewrite Heqb. reflexivity.
+    erewrite sem_filter_in_map in H9. rewrite H9. right. apply Eq_Reflexive.
+    apply H1. apply H3. apply H4. apply H10. apply H1. apply H2. apply H1. apply H2.
+  - assert (Bounded right lb ub). rewrite H7. eapply partitionWithKey_spec. apply H1.
+    apply H2. intros. apply H10. intros. simpl. apply H11. apply H10.
+  - assert (Bounded left lb ub). rewrite H6. eapply partitionWithKey_spec. apply H1.
+    apply H2. intros. simpl. apply H10. intros. apply H11. apply H10.
+  - apply H1.
+Qed. 
+
+Lemma lookup_union_None: forall key (m1: Map e a) m2 lb ub,
+  Bounded m1 lb ub ->
+  Bounded m2 lb ub ->
+  lookup key m1 = None /\ lookup key m2 = None <-> lookup key (union m1 m2) = None.
+Proof.
+  intros. split; intros.
+  - applyDesc union_Desc. erewrite lookup_spec in H1. erewrite lookup_spec in H1. destruct H1.
+    specialize (Hsem key). rewrite H1 in Hsem. rewrite H2 in Hsem. erewrite lookup_spec. 
+    apply Hsem. apply HB. apply H0. apply H.
+  - erewrite lookup_spec in H1. erewrite sem_union_equiv in H1. erewrite lookup_spec.
+    erewrite lookup_spec. unfold sem_union in H1. destruct (sem m1 key) eqn : ?.
+    inversion H1. destruct (sem m2 key). inversion H1. split; reflexivity.
+    apply H0. apply H. apply H. apply H0. applyDesc union_Desc. apply HB.
+Qed.
+
+Lemma lookup_difference_in_snd: forall key m1 m2 value lb ub,
+  Bounded m1 lb ub ->
+  Bounded m2 lb ub ->
+  lookup key m2 = Some value ->
+  lookup key (difference m1 m2) = None.
+Proof.
+  intros. eapply difference_Desc. apply H. apply H0. intros.
+  specialize (H5 key). erewrite lookup_spec in H1. rewrite H1 in H5.
+  simpl in H5. erewrite lookup_spec. apply H5. apply H2. apply H0.
+Qed.
+
+Lemma lookup_difference_not_in_snd: forall key m1 m2 lb ub,
+  Bounded m1 lb ub ->
+  Bounded m2 lb ub ->
+  lookup key m2 = None ->
+  lookup key (difference m1 m2) = lookup key m1.
+Proof.
+  intros. eapply difference_Desc. apply H. apply H0. intros.
+  erewrite lookup_spec in H1. specialize (H5 key). rewrite H1 in H5.
+  simpl in H5. erewrite lookup_spec. erewrite lookup_spec. apply H5.
+  apply H. apply H2. apply H0.
+Qed.
+
+(*This is not true for Maps as it is for IntMaps, since we may have rebalancing. But the
+maps will be equal according to Haskell*)
+Lemma delete_commute: forall `{EqLaws a} k1 k2 m lb ub,
+  Bounded m lb ub ->
+  delete k1 (delete k2 m) == delete k2 (delete k1 m) = true.
+Proof.
+  intros. eapply delete_Desc. 
+  - applyDesc delete_Desc. apply HB.
+  - intros. eapply delete_Desc.
+    + applyDesc delete_Desc. apply HB.
+    + intros. eapply weak_equals_spec. apply H2. apply H5. intros.
+      specialize (H4 i). specialize (H7 i). rewrite H4. rewrite H7.
+      eapply delete_Desc. apply H1. intros. eapply delete_Desc. apply H1.
+      intros. specialize (H10 i). specialize (H13 i). rewrite H10. rewrite H13.
+      destruct (i == k1) eqn : ?; (destruct (i == k2); apply Eq_Reflexive).
+Qed.
+
+Lemma intersection_empty: forall m1 m2 lb ub,
+  Bounded m1 lb ub ->
+  Bounded m2 lb ub ->
+  m1 = empty ->
+  null (intersection m1 m2) = true.
+Proof.
+  intros. applyDesc intersection_Desc. assert (forall i, sem m1 i = None).
+  intros. rewrite H1. reflexivity. setoid_rewrite H2 in Hsem.
+  assert (forall i, sem s i = None). intros i. rewrite Hsem. destruct (sem m2 i); reflexivity.
+  destruct s. 
+  - specialize (H3 e0). simpl in H3. destruct (sem s2 e0). inversion H3. rewrite Eq_Reflexive in H3.
+    inversion H3. 
+  - reflexivity.
+Qed. 
+
+Lemma sem_intersection: forall m1 m2 key lb ub,
+  Bounded m1 lb ub ->
+  Bounded m2 lb ub ->
+  sem (intersection m1 m2) key = sem m1 key &&& sem m2 key.
+Proof.
+  intros. applyDesc intersection_Desc. apply Hsem.
+Qed.
+
+Lemma null_empty_iff: forall (m: Map e a),
+  null m = true <-> m = empty.
+Proof.
+  intros; split; intros.
+  - destruct m. inversion H. reflexivity.
+  - rewrite H. reflexivity.
+Qed.
+
+Lemma sem_insert: forall m1 key value lb ub i,
+  Bounded m1 lb ub ->
+  isLB lb key = true ->
+  isUB ub key = true ->
+  sem (insert key value m1) i = SomeIf (i == key) value ||| sem m1 i.
+Proof.
+  intros. applyDesc insert_Desc. unfold SomeIf. apply Hsem.
+Qed.
+
+(*Have to add hypotheses that key are between bounds so that (insert key value m2) is still Bounded*)
+Lemma null_intersection_non_member: forall m1 m2 key value lb ub,
+  Bounded m1 lb ub ->
+  Bounded m2 lb ub ->
+  isLB lb key = true ->
+  isUB ub key = true ->
+  null (intersection m1 (insert key value m2)) = true <->
+  member key m1 = false /\ null (intersection m1 m2) = true.
+Proof.
+  intros. split; intros.
+  - applyDesc intersection_Desc. rewrite null_empty_iff in H3. rewrite <- empty_no_elts in H3.
+    assert (forall i, sem m1 i &&& sem (insert key value m2) i = None). intros.
+    erewrite <- sem_intersection. apply H3. apply H. applyDesc insert_Desc. 
+    assert (forall i, sem m1 i &&& (SomeIf (i == key) value ||| sem m2 i) = None).
+    intros. erewrite <- sem_insert. apply H4. apply H0. assumption. assumption. 
+    assert (A:=H5). specialize (H5 key). destruct (sem m1 key) eqn : ?.
+    rewrite Eq_Reflexive in H5. simpl in H5. inversion H5. split.
+    + erewrite <- notMember_spec in Heqo. unfold notMember in Heqo. rewrite negb_true_iff in Heqo.
+      apply Heqo. apply H.
+    + assert (forall i, sem s i = None). intros. specialize (Hsem i). rewrite Hsem. specialize (A i).
+      destruct (sem m1 i). unfold ando in *. destruct (sem m2   i) eqn : ?.
+      destruct (i == key); inversion A. reflexivity.
+      destruct (sem m2 i); reflexivity.
+      rewrite null_empty_iff. apply empty_no_elts. apply H6.
+  - applyDesc insert_Desc. applyDesc intersection_Desc. destruct H3. setoid_rewrite Hsem in Hsem0.
+    rewrite null_empty_iff in H4. rewrite <- empty_no_elts in H4. 
+    setoid_rewrite (sem_intersection m1 m2 _ lb ub H H0) in H4. 
+    assert (forall i, sem s0 i = None). { intros. destruct (i == key) eqn : ?.
+    - assert (sem m1 i = None). erewrite <- notMember_spec. unfold notMember.
+      assert (forall a b, a == b = true -> member a m1 = member b m1). { intros.
+      destruct (member b m1) eqn : ?. erewrite member_spec. erewrite member_spec in Heqb0.
+      destruct Heqb0. exists x. erewrite sem_resp_eq. apply H6. apply H5. apply H.
+      apply H. rewrite non_member_lookup. rewrite non_member_lookup in Heqb0.
+      erewrite lookup_spec. erewrite lookup_spec in Heqb0. erewrite sem_resp_eq.
+      apply Heqb0. apply H5. apply H. apply H. apply H. apply H. }
+      apply H5 in Heqb. rewrite Heqb. rewrite H3. reflexivity. apply H. 
+      specialize (Hsem0 i). rewrite H5 in Hsem0. rewrite Heqb in Hsem0. simpl in Hsem0.
+      apply Hsem0.
+    - specialize (Hsem0 i). rewrite Heqb in Hsem0. simpl in Hsem0.
+      rewrite H4 in Hsem0. apply Hsem0. }
+      rewrite null_empty_iff. apply empty_no_elts. apply H5.
+Qed.
+
+Lemma difference_sem: forall m1 m2 lb ub key,
+  Bounded m1 lb ub ->
+  Bounded m2 lb ub ->
+  sem (difference m1 m2) key = diffo (sem m1 key) (sem m2 key).
+Proof.
+  intros. eapply difference_Desc. apply H. apply H0. intros.
+  rewrite H4. reflexivity.
+Qed. 
+
+Lemma disjoint_difference: forall m1 m2 m3 lb ub,
+  Bounded m1 lb ub ->
+  Bounded m2 lb ub ->
+  Bounded m3 lb ub ->
+  null (intersection m2 m3) = true ->
+  null (difference m1 m2) = true ->
+  null (intersection m1 m3) = true.
+Proof.
+  intros. applyDesc intersection_Desc. rewrite null_empty_iff in H2.
+  rewrite null_empty_iff in H3. rewrite <- empty_no_elts in H2.
+  rewrite <- empty_no_elts in H3. setoid_rewrite (sem_intersection m2 m3 _ lb ub H0 H1) in H2.
+  setoid_rewrite (difference_sem m1 m2 lb ub _ H H0) in H3.
+  assert (forall i, sem s i = None). { intros. specialize (Hsem i).
+  specialize (H2 i). specialize (H3 i). rewrite Hsem. destruct (sem m1 i).
+  destruct (sem m3 i). simpl in H2. rewrite H2 in H3. simpl in H3. inversion H3.
+  simpl. reflexivity. destruct (sem m3 i). simpl. reflexivity. simpl. reflexivity. }
+  rewrite null_empty_iff. eapply empty_no_elts. apply H4.
+Qed. 
 
 End WF.
 (*Could not find [ordered], [valid], [validsize] or similar in Data.Map*)
@@ -5926,12 +6852,6 @@ Proof.
   - simpl. apply Eq_Reflexive.
 Qed.
 
-
-Lemma eq_coq_implies_haskell : forall {a} `{EqLaws a} (x y : a),
-  x = y -> x == y = true.
-Proof.
-  intros. subst. apply Eq_Reflexive.
-Qed.
 
 (*Haskell equality version of [map_none_spec] *)
 Lemma map_none_spec_haskell:
@@ -6317,397 +7237,112 @@ Proof.
   rewrite oro_assoc. apply Eq_Reflexive.
 Qed.
 
-(*Skipping Monoid for now - causes Coq to freeze*)
+(** ** Verification of [Monoid] *)
 
+Global Program Instance Monoid_WF : Monoid (WFMap e a) := fun _ k => k
+  {| mempty__   := @mempty (Map e a) _ _
+   ; mappend__  := @mappend (Map e a) _ _
+   ; mconcat__  xs := @mconcat (Map e a) _ _ (List.map (fun x => unpack x) xs)
+  |}.
+Next Obligation.
+  destruct x as [s1 HB1], x0 as [s2 HB2]. simpl. unfold mappend.
+  unfold_Monoid_Map.
+  eapply union_Desc; try eassumption. intuition.
+Qed.
+Next Obligation.
+  unfold mconcat.
+  unfold_Monoid_Map.
+  eapply unions_Desc.
+  * induction xs.
+    + constructor.
+    + destruct a as [s HB]. simpl. constructor. apply HB. apply IHxs.
+  * intros. assumption.
+Qed.
+Next Obligation.
+  unfold_Monoid_Set.
+  eapply empty_Desc.
+  eauto.
+Qed.
+
+(*Skipping Monoid for now - causes Coq to freeze*)
+Lemma map_preserves_size: forall {b} {c} (m : Map e b) (f : b -> c) lb ub,
+  Bounded m lb ub ->
+  size m = size (map f m).
+Proof.
+  intros. inversion H.
+  - simpl. reflexivity.
+  - simpl. reflexivity.
+Qed.
+
+Lemma map_bounded: forall {b} {c} (m : Map e b) (f: b -> c) lb ub,
+  Bounded m lb ub ->
+  Bounded (map f m) lb ub.
+Proof.
+  intros. induction H.
+  - simpl. apply BoundedTip.
+  - simpl. apply BoundedBin. apply IHBounded1. apply IHBounded2. apply H1.
+    apply H2. erewrite <- map_preserves_size. erewrite <- map_preserves_size. apply H3.
+    apply H0. apply H. erewrite <- map_preserves_size. erewrite <- map_preserves_size.
+    apply H4. apply H0. apply H.
+Qed. 
+
+Lemma map_preserves_WF : forall {b} {c} (m : Map e b) (f : b -> c),
+  WF m -> WF (map f m).
+Proof. 
+  intros. unfold WF in *. apply map_bounded. apply H.
+Qed. 
+
+
+Definition Functor__Map_fmap 
+   : forall {a} {b}, (a -> b) -> (Map e) a -> (Map e) b :=
+  fun {a} {b} => fun f m => map f m.
+
+Local Definition Functor__map_op_zlzd__
+   : forall {a} {b}, a -> Map e b -> Map e a :=
+  fun {a} {b} => Functor__Map_fmap ∘ const.
+
+Lemma const_WF: forall {b} {a: Type} (x : a) (m: Map e b),
+  WF m -> WF (map (const x) m).
+Proof.
+  intros. apply map_preserves_WF. apply H. 
+Qed.
+
+
+Global Program Instance Functor_Map : Functor (WFMap e) :=
+  fun _ k => 
+  k {| GHC.Base.fmap__ := fun {a} => @fmap (Map e) _ _ ;
+        GHC.Base.op_zlzd____ := fun {a} {b} x => @fmap (Map e) _ b a (@const a b _) |}.
+Next Obligation.
+  unfold proj1_sig. destruct x1. apply map_preserves_WF. apply w.
+Qed.
+Next Obligation.
+  unfold proj1_sig. destruct x0. apply const_WF. apply w.
+Qed.
+
+Set Bullet Behavior "Strict Subproofs".
+
+Global Instance FunctorLaws_MapWF: FunctorLaws (WFMap e).
+  constructor.
+  - intros. destruct x. unfold fmap. unfold fmap__.  unfold Functor_Map. 
+    apply ProofIrrelevance.ProofIrrelevanceTheory.subset_eq_compat. unfold proj1_sig.
+    unfold fmap. unfold fmap__. unfold Functor__Map. unfold Internal.Functor__Map_fmap.
+    induction w. 
+    + simpl. reflexivity.
+    + simpl. rewrite IHw1. rewrite IHw2. reflexivity.
+  - intros. destruct x. unfold fmap in *. unfold fmap__ in *.
+    unfold Functor_Map in *. apply ProofIrrelevance.ProofIrrelevanceTheory.subset_eq_compat.
+    unfold proj1_sig in *. unfold fmap. unfold Functor__Map. unfold fmap__. 
+    unfold Internal.Functor__Map_fmap. simpl. induction w.
+    + simpl. reflexivity.
+    + simpl. rewrite IHw1. rewrite IHw2. reflexivity.
+Qed. 
 
 End TypeClassLaws.
 
 
 Section ContainerAxioms.
 Context {e : Type} {a : Type} {HEq : Eq_ e} {HOrd : Ord e} {HEqLaws : EqLaws e}  {HOrdLaws : OrdLaws e}.
-(*The following theorems are the axioms from ContainerAxioms and have no clear analogue in SetProofs*)
 
-(*Simpler definition of lookup*)
-Fixpoint lookup' (key : e) (map : Map e a) : option a :=
-  match map with
-  | Tip => None
-  | Bin sz k1 v1 lt rt => match compare key k1 with
-                          | Eq => Some v1 
-                          | Lt => lookup' key lt 
-                          | Gt => lookup' key rt
-                          end
- end.  
-
-(*Prove the two definitions are equivalent*)
-Lemma lookup_lookup'_equiv : forall  (key : e) (map : Map e a),
-    lookup key map = lookup' key map.
-Proof.
-  intros. induction map.
-  - simpl. destruct (compare key k); try (reflexivity); assumption.
-  - simpl. reflexivity.
-Qed.  
-
-(*This lemma says that if two keys are equal, then the result of member is the same when either is called*)
-Lemma member_eq: forall {a : Type} (n : e) (n' : e) (m : Map e a),
-  n == n' = true ->
-  member n m = member n' m.
-Proof.
-  intros. induction m.
-   - simpl. destruct (compare n k) eqn : E.
-    + rewrite Ord_compare_Eq in E.  
-      apply Lemmas.Eq_trans_l  with(z:=k) in H.
-      rewrite E in H. symmetry in H. rewrite <- Ord_compare_Eq in H.
-      rewrite H. reflexivity.
-    + rewrite Ord_compare_Lt in E. 
-      apply Lemmas.Eq_le_r with(z:=k) in H. rewrite E in H. 
-      symmetry in H. rewrite <- Ord_compare_Lt in H. 
-      rewrite H. assumption.
-    + rewrite Ord_compare_Gt in E. apply Lemmas.Eq_le_l with (z:=k) in H.
-      rewrite E in H. symmetry in H. rewrite <- Ord_compare_Gt in H.
-      rewrite H. assumption.
-  - simpl. reflexivity.
-Qed.
-
-(*If we insert a (key, value) in a map, then looking up the key gives the value*)
-Lemma lookup_insert : forall `{Eq_ a} `{EqLaws a} (key: e) (value : a) (map : Map e a) lb ub,
-  Bounded map lb ub ->
-  isLB lb key = true ->
-  isUB ub key = true ->
-  lookup' key (insert' key value map)  == Some value = true.
-Proof.
-  intros. pose proof (insert_Desc key value map lb ub) as H5. eapply H5 in H2. 
-  unfold Desc in H2. destruct H2 with(P:= fun (map1 : Map e a) => lookup' key map1 == Some value = true).
-  - intros. 
-  assert (sem s key = (if _GHC.Base.==_ key key then Some value else None) ||| sem map key). { apply H8. }
-  rewrite Eq_Reflexive in H9. simpl in H9. eapply lookup_spec in H6. 
-  rewrite <- H6 in H9. rewrite <- lookup_lookup'_equiv. rewrite H9. apply Eq_Reflexive.
-  - rewrite insert_insert'. reflexivity.
-  - assumption.
-  - assumption.
-Qed.
-
-(*If we lookup a key key1, the result is the same regardless of whether or not we have inserted key2 
-(a different key than key1)*)
-Lemma lookup_insert_neq : forall `{Eq_ a} `{EqLaws a} (key1: e) (key2: e) (value : a) (map : Map e a) lb ub,
-  Bounded map lb ub ->
-  isLB lb key2 = true ->
-  isUB ub key2 = true ->
-  key1 == key2 = false -> 
-  lookup' key1 (insert' key2 value map) = lookup' key1 map.
-Proof.
-  intros. pose proof (insert_Desc key2 value map lb ub) as H6. assert (A := H2). eapply H6 in H2. 
-  unfold Desc in H2. destruct H2 with(P:= fun (map1 : Map e a) => lookup' key1 map1 = lookup' key1 map).
-  - intros. assert (sem s key1 = (if _GHC.Base.==_ key1 key2 then Some value else None) ||| sem map key1).
-    { apply H9. } rewrite H5 in H10. simpl in H10. 
-  eapply lookup_spec in H7. rewrite <- H7 in H10. eapply lookup_spec in A. rewrite <- H10 in A.
-  rewrite <- lookup_lookup'_equiv. rewrite <- A. rewrite lookup_lookup'_equiv. reflexivity.
-  - rewrite insert_insert'. reflexivity.
-  - assumption.
-  - assumption.
-Qed.
- 
- 
-(*States that if we check for key1 in the map in which we have inserted key2, then either
-key1 was already in the map, or key1 == key2*)
-Lemma member_insert: forall key1 key2 value (map: Map e a) lb ub,
-  Bounded map lb ub ->
-  isLB lb key2 = true ->
-  isUB ub key2 = true ->
-  member key1 (insert' key2 value map) = (key1 == key2) || member key1 map. 
-Proof.
-  intros. pose proof (insert_Desc key2 value map lb ub) as H5. assert (A := H). eapply H5 in H.
-  unfold Desc in H. 
-  destruct H with(P:= fun (map1 : Map e a) => member key1 map1 = (key1 == key2) || member key1 map).
-  - intros. assert(sem s key1 = (if _GHC.Base.==_ key1 key2 then Some value else None) ||| sem map key1).
-    { apply H4. } destruct (key1 == key2) eqn : ?. simpl in H6. 
-    eapply member_spec in H2. destruct H2. assert (member key1 s = true). { apply H7. exists value.
-    assumption. } rewrite H8. simpl. reflexivity. 
-    eapply member_spec in H2. destruct H2. simpl in H6. destruct (sem s key1) eqn : E.
-    + assert (member key1 s = true). { apply H7. exists a0. assumption. } 
-      eapply member_spec in A. destruct A. assert (member key1 map =true). {
-      apply H10. exists a0. symmetry in H6. assumption. }
-      rewrite H11. simpl. assumption.
-    + simpl. eapply member_spec in A. destruct A. assert (member key1 s = false). {
-      apply contrapositive in H2. destruct (member key1 s)  eqn : ?. contradiction.
-      reflexivity. intro. destruct H10. rewrite H10 in E. discriminate E. }
-      assert (member key1 map = false). { apply contrapositive in H8. 
-      destruct (member key1 map) eqn : ?. rewrite Heqb0 in H8. contradiction.
-      reflexivity. intro. destruct H11. rewrite H11 in H6. discriminate H6. }
-      rewrite H10. rewrite H11. reflexivity.
-  - rewrite insert_insert'. reflexivity.
-  - assumption.
-  - assumption.
-Qed.
-
-(*If we lookup a key that is deleted, we should get None*)
-Lemma delete_eq : forall key (map : Map e a) lb ub,
-  Bounded map lb ub ->
-  lookup key (delete key map) = None.
-Proof.
-  intros. pose proof (delete_Desc key map lb ub) as H2. eapply H2 in H. unfold Desc in H.
-  destruct H with(P:= fun (map1 : Map e a) => lookup key map1 = None).
-  - intros. eapply lookup_spec in H0.
-    assert (sem s key = (if _GHC.Base.==_ key key then None else sem map key)). { apply H3. }
-    rewrite Eq_Reflexive in H4. rewrite H4 in H0. assumption. 
-  - reflexivity.
-Qed.
-
-(*If we delete a key key2 and then lookup a different key key1, then it should be the same regardless of
-whether or not key2 was deleted.*)
-Lemma delete_neq : forall key1 key2 (map : Map e a) lb ub,
-  Bounded map lb ub ->
-  key1 == key2 = false ->
-  lookup key1 (delete key2 map) = lookup key1 map.
-Proof.
-  intros. pose proof(delete_Desc key2 map lb ub) as H1. assert(A:= H). eapply H1 in H.
-  unfold Desc in H. destruct H with(P:= fun (map1 : Map e a) => lookup key1 map1 = lookup key1 map).
-  - intros. assert (sem s key1 = (if _GHC.Base.==_ key1 key2 then None else sem map key1)). { apply H4. }
-    rewrite H0 in H5. eapply lookup_spec in H2. eapply lookup_spec in A. rewrite H5 in H2.
-    rewrite <- H2 in A. symmetry. assumption.
-  - reflexivity.
-Qed. 
-
-(*Same as above but for member*)
-Lemma member_delete_neq: forall key1 key2 (map: Map e a) lb ub,
-  Bounded map lb ub ->
-  key1 == key2 = false ->
-  member key2 (delete key1 map) = member key2 map.
-Proof.
-  intros. pose proof(delete_Desc key1 map lb ub) as H1. assert(A:=H). eapply H1 in H.
-  unfold Desc in H. destruct H with(P:= fun(map1 : Map e a) => member key2 map1 = member key2 map).
-  - intros. assert (sem s key2 = (if _GHC.Base.==_ key2 key1 then None else sem map key2)). { apply H4. }
-    rewrite Lemmas.Eq_neq_sym in H5. eapply member_spec in H2. eapply member_spec in A.
-    destruct (sem s key2)  eqn : ?.
-    + destruct A. assert (member key2 map = true). { apply H7. exists a0. symmetry. assumption. }
-      destruct H2. assert (member key2 s = true). { apply H9. exists a0. assumption. }
-      rewrite H8. rewrite H10. reflexivity.
-    + destruct A. destruct H2. apply contrapositive in H6. apply contrapositive in H2.
-      destruct (member key2 s) eqn : ?. contradiction. destruct (member key2 map) eqn : ?.
-      contradiction. reflexivity. intro. destruct H9. rewrite H9 in Heqo. discriminate Heqo.
-      intro. destruct H9. rewrite H9 in H5. discriminate H5.
-    + assumption.
- - reflexivity.
-Qed.
-
-(*States that if a key is not in the map, then looking it up will give None, and vice versa. *)
-Lemma non_member_lookup :
-  forall key (map: Map e a) lb ub,
-  Bounded map lb ub ->
-  (member key map = false) <-> (lookup key map = None).
-Proof.
-  intros. assert(A:=H). eapply member_spec in H.  destruct (member key map) eqn : E.
-  - destruct H. apply H in E. destruct E. eapply lookup_spec in A. rewrite H1 in A.
-    rewrite A.  split; intros; discriminate H2. 
-  - split; intros. destruct H. apply contrapositive in H1. destruct (lookup key map) eqn :?.
-    + unfold not in H1. destruct H1. exists a0. eapply lookup_spec in A.
-      rewrite Heqo in A. symmetry. assumption.
-    + reflexivity. 
-    + intro. rewrite H2 in E. discriminate E.
-    + reflexivity.
-Qed.
-
-(*If two keys are equal (according to the Eq typeclass), then their values in 
-a map are equal*)
-Lemma lookup_eq : forall k k' (m : Map e a),
-    k == k' = true ->
-    lookup k m = lookup k' m.
-Proof.
-  intros. induction m.
-  - simpl. destruct (compare k k0) eqn : E.
-    + rewrite Ord_compare_Eq in E. apply Lemmas.Eq_trans_l with(z:=k0) in H .
-      rewrite E in H. symmetry in H. rewrite <- Ord_compare_Eq in H.
-      rewrite H. reflexivity.
-    + rewrite Ord_compare_Lt in E. apply Lemmas.Eq_le_r with (z:= k0) in H.
-      rewrite E in H. symmetry in H. rewrite <- Ord_compare_Lt in H.
-      rewrite H. assumption.
-    + rewrite Ord_compare_Gt in E. apply Lemmas.Eq_le_l with (z:=k0) in H.
-      rewrite E in H. symmetry in H. rewrite <- Ord_compare_Gt in H.
-      rewrite H. assumption.
-  - simpl. reflexivity.
-Qed.
-
-(*This follows almost immediately from member_spec*)
-Lemma member_lookup : 
-  forall key (map: Map e a) lb ub,
-  Bounded map lb ub -> 
-  (member key map = true) <-> (exists value, lookup key map = Some value).
-Proof.
-  intros. assert(A:=H). eapply member_spec in A. eapply lookup_spec in H.
-  rewrite <- H in A. apply A.
-Qed. 
-
-(** ** Verification of [null] *)
-Lemma null_empty: 
-    @null e a empty = true.
-Proof.
-  unfold null. simpl. reflexivity.
-Qed. 
-
-(*A key is a member of the union of two maps whenever it is a member of at least one of the maps*)
-Lemma member_union :
-  forall key (map1: Map e a) map2 lb ub,
-  Bounded map1 lb ub ->
-  Bounded map2 lb ub ->
-  member key (union map1 map2) = member key map2 || member key map1.
-Proof.
-  intros. pose proof(union_Desc map1 map2 lb ub) as H1. assert (A:=H).
-  eapply H1 in H. unfold Desc' in H. 
-  destruct H with(P:= fun (m : Map e a) => member key m = member key map2 || member key map1).
-  - intros. assert (sem s key = sem map1 key ||| sem map2 key). { apply H4. }
-    eapply member_spec in H2. eapply member_spec in A.
-    unfold oro in H5. destruct (sem map1 key) eqn : ?.
-    + assert (member key s = true). { apply H2. exists a0. assumption. }
-      assert (member key map1 = true). { apply A. exists a0. assumption. }
-      rewrite H6. rewrite H7. symmetry. rewrite orb_true_iff. right. reflexivity.
-    + destruct A. destruct H2. eapply member_spec in H0. destruct H0.
-      destruct (sem s key) eqn : ?.
-      * assert (member key s = true). { apply H8. exists a0. reflexivity. }
-        assert (member key map2 = true). { apply H9. exists a0. symmetry. assumption. }
-        rewrite H10. rewrite H11. simpl. reflexivity.
-      * apply  contrapositive in H6. apply contrapositive in H2. apply contrapositive in H0.
-        destruct (member key s). contradiction. destruct (member key map1). contradiction.
-        destruct (member key map2). contradiction. simpl. reflexivity.
-        intro. destruct H10. rewrite H10 in H5. discriminate H5.
-        intro. destruct H10. discriminate H10.
-        intro. destruct H10. rewrite H10 in Heqo. discriminate Heqo.
-  - reflexivity.
-  - assumption.
-Qed. 
-
-(*The union of a map with the empty map (in both directions) is itself*)
-Lemma union_nil_l : forall (map: Map e a) ub lb,
-  Bounded map ub lb ->
-  union empty map = map.
-Proof.
-  intros.  induction H.
-  - reflexivity.
-  - simpl. destruct s1 eqn : ?. reflexivity.
-    destruct s2 eqn : ?. reflexivity.
-    unfold insertR. unfold singleton. simpl in H3.
-    rewrite H3. reflexivity.
-Qed.
-
-Lemma union_nil_r : forall (map: Map e a) ub lb,
-  Bounded map ub lb ->
-  union map empty = map.
-Proof.
-  intros. induction H.
-  - simpl. reflexivity.
-  - simpl. destruct s1. reflexivity. destruct s2. reflexivity. reflexivity.
-Qed.
-
-(*The difference between a map and itself is the empty map*)
-Lemma difference_self: forall (map: Map e a) lb ub,
-  Bounded map lb ub ->
-  difference map map = empty.
-Proof.
-  intros. pose proof(difference_Desc map map lb ub) as H1. assert(A:=H). 
-  eapply H1 with(P:= fun(map1 : Map e a) => map1 = empty) in A .
-  - assumption.
-  - assumption.
-  - intros. assert ( forall i, sem s i = None). {
-    intros. assert (sem s i = diffo (sem map i) (sem map i)). { apply H4. }
-    unfold diffo in H5. destruct (sem map i) eqn : ?.
-    assumption. assumption. }
-    rewrite sem_false_nil in H5. assumption.
-Qed.
-
-(*The difference of a map with the empty map is itself*)
-Lemma difference_nil_r: forall `{Eq_ a} `{EqLaws a} (B : Type) (map: Map e a) lb ub,
-  Bounded map lb ub ->
-  difference map (@empty e B) = map.
-Proof.
-  intros. inversion H2.
-  - simpl. reflexivity.
-  - simpl. reflexivity.
-Qed.
-
-(*The difference of the empty map with any map is empty*)
-Lemma difference_nil_l: forall `{Eq_ a} `{EqLaws a} (B : Type) (map: Map e a) lb ub (key : e),
-  Bounded map lb ub ->
-  difference (@empty e B) map = empty.
-Proof.
-  intros. inversion H2.
-  - simpl. reflexivity.
-  - simpl. unfold empty. reflexivity.
-Qed.
-
-(*Follows from sem_inside, says that if a key is in a map, it is between the bounds*)
-Lemma keys_inside_bounds : forall (map: Map e a) key lb ub,
-  Bounded map lb ub ->
-  member key map = true ->
-  isLB lb key = true /\ isUB ub key = true .
-Proof.
-  intros. eapply member_spec in H0. destruct H0.
-  eapply sem_inside. apply H. apply H0. apply H.
-Qed.
-
-(*If a key is in a map, the difference of the singleton map containing only that key
-and the original map is empty*)
-Lemma difference_Tip_member: forall (map: Map e a) (key :e) lb ub,
-  Bounded map lb ub ->
-  member key map = true ->
-  forall (value : a), difference (singleton key value) map = empty.
-Proof.
-  intros. assert (A:=H). induction H.
-  - discriminate H0.
-  - pose proof(difference_Desc (singleton key value) (Bin sz x v s1 s2) lb ub) as H6. 
-  eapply H6 with(P:=(fun map1 => map1 = empty)). eapply BoundedBin. apply BoundedTip.
-  apply BoundedTip. eapply keys_inside_bounds in H0. destruct H0.
-  apply H0. apply A. eapply keys_inside_bounds in H0. destruct H0. apply H7.
-  apply A. simpl. reflexivity. simpl. unfold balance_prop. simpl. omega. apply A.
-  intros.  eapply member_spec in H0. destruct H0.
-  assert (forall i : e, sem s i = None). {
-  intros i. assert (sem s i = diffo (sem (singleton key value) i) (sem (Bin sz x v s1 s2) i)). {
-  apply H10. } destruct (i == key) eqn : ?.
-  + simpl in H11. rewrite Heqb in H11. simpl in H11. 
-    assert (sem s1 i = sem s1 key). { apply sem_resp_eq. assumption. } 
-    assert (sem s2 i = sem s2 key). { apply sem_resp_eq. assumption. } 
-    assert ((i == x) = (key == x)). { eapply Lemmas.Eq_trans_l. assumption. }
-    rewrite H12 in H11. rewrite H14 in H11. rewrite H13 in H11. simpl in H0.
-    rewrite H0 in H11. simpl in H11. apply H11. 
-  + simpl in H11. rewrite Heqb in H11. simpl in H11. unfold diffo in H11. 
-    destruct (sem s1 i ||| SomeIf (_GHC.Base.==_ i x) v ||| sem s2 i) eqn : ?.
-    assumption. assumption. }
-    rewrite <- sem_false_nil. assumption. apply A.
-Qed.
-
-(*Might have to put this back in WF
-Lemma difference_Tip_non_member: forall `{Eq_ a} `{EqLaws a} (map: Map e a) (key :e) lb ub,
-  Bounded map lb ub ->
-  isUB ub key = true ->
-  isLB lb key = true ->
-  member key map = false ->
-  forall (value : a), difference (singleton key value) map == (singleton key value) = true.
-Proof.
-  intros. pose proof(difference_Desc (singleton key value) map lb ub) as H6. 
-  assert(A:=H). assert (Bounded (singleton key value) lb ub). { unfold singleton.
-  apply BoundedBin. apply BoundedTip. apply BoundedTip. assumption. assumption. simpl.
-  reflexivity. simpl. unfold balance_prop. omega. } 
-  eapply H6 with(P:=(fun map1 => map1 == singleton key value = true)). assumption.
-  assumption. intros.
-  simpl in H8.
-  pose proof(@member_spec map lb ub key) as H12. assert(A1:=A). apply H12 in A.
-  destruct A. apply contrapositive in H14. assert (sem map key = None). {
-  unfold not in H14. destruct (sem map key). destruct H14. exists a0. reflexivity.
-  reflexivity. }
-  assert (forall i, i == key = false -> sem s i = None). {
-  intros. assert (sem s i = diffo (SomeIf (_GHC.Base.==_ i key) value ||| None) (sem map i)). {
-  apply H11. } rewrite H16 in H17. simpl in H17. unfold diffo in H17. destruct (sem map i); assumption.
-  }
-  assert (sem s key = Some value). { 
-  assert (sem s key = diffo (SomeIf (_GHC.Base.==_ key key) value ||| None) (sem map key)). {
-  apply H11. } rewrite Eq_Reflexive in H17. simpl in H17. rewrite H15 in H17. simpl in H17.
-  assumption. }
-  assert (forall i, sem s i = SomeIf (i == key) value). {
-  intros. destruct (i == key) eqn : ?. { simpl. rewrite <- (sem_resp_eq s key).
-  assumption. apply Eq_Symmetric. apply Heqb. }
-  { simpl. apply H16 in Heqb. assumption. }
-  } applyDesc singleton_Desc. assert (forall i, sem s i = sem s0 i). {
-    intros. rewrite H18. rewrite Hsem. reflexivity. }
-    eapply strong_eq1. apply H8. apply HB. apply H19. intro. rewrite H15 in H5.
-    discriminate H5. intros. apply H2.
-Qed.*)
 End ContainerAxioms.
 
 
